chore: clean up file

Iris/Iris/Algebra/OFE.lean
@@ -275,6 +275,12 @@ infixr:25 " -c> " => ContractiveHom
 instance [OFE α] [OFE β] : CoeFun (α -c> β) (fun _ => α → β) := ⟨fun x => x.toHom.f⟩
 instance [OFE α] [OFE β] (f : α -c> β) : Contractive f := f.contractive
 
+-- TODO: I propose this definition, to allow doing `f.toContractiveHom` to infer the necessary
+-- instances to make `f : α → β` into a `α -c> β`.
+def _root_.Function.toContractiveHom (f : α → β)[OFE α][OFE β][ι : OFE.Contractive f] : α -c> β where
+  f := f
+  contractive := ι
+
 theorem InvImage.equivalence {α : Sort u} {β : Sort v}
     {r : β → β → Prop} {f : α → β} (H : Equivalence r) : Equivalence (InvImage r f) where
   refl _ := H.refl _
@@ -1770,4 +1776,3 @@ theorem OFE.cast_dist [Iα : OFE α] [Iβ : OFE β] {x y : α}
     (Ht : α = β) (HIt : Iα = Ht ▸ Iβ)  (H : x ≡{n}≡ y) :
     (Ht ▸ x) ≡{n}≡ (Ht ▸ y) := by
   subst Ht; subst HIt; exact H
-
